L5_to_L6 now also converts the inductive environment into the constructor environment required for further phases of the compile. Changed the L6 language instance to include the constructor environment

theories/L6_PCPS/L5_to_L6.v
@@ -12,6 +12,7 @@
 
 Require Import Coq.ZArith.ZArith.
 Require Import Coq.ZArith.Znumtheory.
+Require Import Coq.Strings.String.
 Require Import ExtLib.Data.List.
 Require Import ExtLib.Data.Bool.
 Require Libraries.Maps.
@@ -20,6 +21,17 @@ Import Nnat.
 Require Import CpdtTactics.
 
 
+(******)
+Add LoadPath "../common" as Common.
+Add LoadPath "../L1g" as L1g.
+Add LoadPath "../L1_QuotedCoq" as L1.
+Add LoadPath "../L1_5_box" as L1_5.
+Add LoadPath "../L2_typeStripped" as L2.
+Add LoadPath "../L3_flattenedApp" as L3.
+Add LoadPath "../L4_deBruijn" as L4.
+(******)
+
+Require Export Common.Common.  (* shared namespace *)
 Require Import ExtLib.Data.List.
 Require Import L4.L4a_to_L5.
 Require Import SquiggleEq.varImplZ.
@@ -44,9 +56,41 @@ Variable kvar_tag : tag.
 Variable rec_tag : tag.
 Variable fun_tag: tag.
 Variable kon_tag: tag.
-                    
-Definition dcon_to_tag:dcon -> cTag :=
-  fun x => N.succ_pos (snd x). (* should probably change dcon to positive in simple_cps *)
+
+
+Definition L5_conId := dcon.
+
+Theorem L5_conId_dec: forall x y:L5_conId, {x = y} + {x <> y}.
+Proof.
+  intros. destruct x,y.
+  assert (H:=inductive_dec i i0).
+  destruct H.
+  - destruct (eq_dec n n0).
+    + subst. left. auto.
+    + right. intro. apply n1. inversion H. auto.
+  - right; intro; apply n1. inversion H; auto.
+Qed.
+    
+Definition L6_conId := cTag.
+Definition d_L6_conId := 1%positive.
+
+Definition conId_map:= list (L5_conId * L6_conId).
+
+
+
+
+Print sumbool.
+
+Fixpoint dcon_to_tag (a:L5_conId) (sig:conId_map) :=
+  match sig with
+    | nil => d_L6_conId
+    | ((cId, tag)::sig') => match L5_conId_dec a cId with
+                              | left _ => tag
+                              | right _ => dcon_to_tag a sig'
+                            end
+  end.
+
+
 
 
 (* returns list of numbers [n, n+m[  and the positive n+m (next available pos) *)
@@ -69,15 +113,16 @@ Fixpoint ctx_bind_proj (r:positive) (m:nat) (n:var) : (exp_ctx * var) :=
   end.
 
 
-Definition t_map := M.t tag.
-Definition t_empty := M.empty tag.
 
-
-Definition get_t (a:M.elt) (sig:t_map) :=
-  match M.get a sig with
-    | None => default_tag
+Definition t_map := M.t iTag.
+Definition t_empty:t_map := M.empty _.
+  
+Fixpoint get_t (n:var) (sig:t_map): iTag :=
+  match M.get n sig with
+    | None => (1%positive)
     | Some v => v
   end.
+
   
 
 
@@ -116,33 +161,40 @@ note : var "1" is taken as error and will be proven not to appear when input is 
 
  *)
 
-Fixpoint convert (e:cps) (sv: s_map) (sk:s_map) (tgm:t_map) (n:var) (*  {struct e } *): exp * var * t_map :=
+(* environment threaded for conversion 
+ conId_map maps the dcon to the right tag pointing to the constructor info (cEnv not passed around)
+ t_map maps var name to their tag, allowing to index applications with the right function tag  
+*)
+Definition conv_env:Type := conId_map *  t_map.
+
+Fixpoint convert (e:cps) (sv: s_map) (sk:s_map) (tgm:conv_env) (n:var) (*  {struct e } *): exp * var * conv_env :=
        match e with
        | Halt_c v => let '(ctx_v, vn, n', tgm) := convert_v v sv sk tgm n in
                          (app_ctx_f ctx_v (Ehalt vn), (Pos.succ n'), tgm)
        | Ret_c k v => let '(ctx_k, kn, n', tgm) := convert_v k sv sk tgm n in
                       let '(ctx_v, vn, n'', tgm) := convert_v v sv sk tgm n' in
-                       (app_ctx_f (comp_ctx_f ctx_k ctx_v) (Eapp  kn (get_t kn tgm) (vn::nil)), n'', tgm)
+                       (app_ctx_f (comp_ctx_f ctx_k ctx_v) (Eapp  kn (get_t kn (snd tgm)) (vn::nil)), n'', tgm)
        | Call_c f k v =>
          let fv := if (varInterface.varClass f):bool then sv else sk in
          let kv := if (varInterface.varClass k):bool then sv else sk in
          let vv := if (varInterface.varClass v):bool then sv else sk in
          (* flipping around so the continuation comes first *)
          let f' := get_s f fv in
-         (Eapp f' (get_t f' tgm) ((get_s k kv)::(get_s v vv)::nil) , n, tgm)
+         (Eapp f' (get_t f' (snd tgm)) ((get_s k kv)::(get_s v vv)::nil) , n, tgm)
          
        | Match_c v bl =>
-         let fix convert_branches (bl:list  ((dcon * nat) * ((list NVar)* cps))) (sv: s_map) (sk:s_map) (tgm:t_map) (r:var)  (n:var)  (* { struct bl } *): (list (cTag * exp) * var * t_map)  :=
+         let fix convert_branches (bl:list  ((dcon * nat) * ((list NVar)* cps))) (sv: s_map) (sk:s_map) (tgm:conv_env) (r:var)  (n:var)  (* { struct bl } *): (list (cTag * exp) * var * conv_env)  :=
              (* {| n -> k, \ n+1 . (let n+2 <- \pi_1 n+1 ... n+m+1 <- \pi_m n+1 in  ce |}  *)
              match bl with
                | nil => ( nil, n, tgm)
                | ((dcn, m),(xs, e))::bl' =>
+                 let lxs := List.length xs in 
                  let '(cbl, n', tgm) := convert_branches bl' sv sk tgm r n in
-                 let (ctx_p, n'') := ctx_bind_proj r m n' in 
-                 let (names, _) := fromN n' m in
+                 let (ctx_p, n'') := ctx_bind_proj r lxs n' in 
+                 let (names, _) := fromN n' lxs in
                  let sv' := set_s_list xs names sv in
                  let '(ce, n''', tgm) :=  convert e sv' sk tgm n'' in
-                 (((dcon_to_tag dcn), (app_ctx_f ctx_p ce))::cbl , n''', tgm) 
+                 (((dcon_to_tag dcn (fst tgm)), (app_ctx_f ctx_p ce))::cbl , n''', tgm) 
              end in
          let '(ctx_v, vn, n', tgm) := convert_v v sv sk tgm n in
          let '(cbls, n'', tgm) := convert_branches bl sv sk tgm vn n' in
@@ -160,7 +212,7 @@ Ret_c M N ->
    App_e m n
 
 *)
-with convert_v (v:val_c) (sv: s_map) (sk: s_map) (tgm:t_map) (n:var) (* { struct v }  *): (exp_ctx * var * var * t_map) :=
+with convert_v (v:val_c) (sv: s_map) (sk: s_map) (tgm:conv_env) (n:var) (* { struct v }  *): (exp_ctx * var * var * conv_env) :=
        match v with
          | Var_c m => (Hole_c, get_s m sv , n, tgm)   (* {| ( Econstr_c n ty var_tag ((nth (N.to_nat m) sv (1%positive))::nil)  Hole_c, Pos.succ n  ) |} *)
          | KVar_c m => (Hole_c, get_s m sk, n, tgm) (* {| ( Econstr_c n ty kvar_tag ((nth (N.to_nat m) sk (1%positive))::nil) Hole_c, Pos.succ n) |} *)
@@ -172,7 +224,7 @@ with convert_v (v:val_c) (sv: s_map) (sk: s_map) (tgm:t_map) (n:var) (* { struct
                          let fds := Fcons n' kon_tag (n::nil) e' Fnil in
                          (Efun1_c fds Hole_c, n',  Pos.succ n', tgm)
          | Con_c dcn lv =>
-           let fix convert_v_list (lv :list val_c) (sv : s_map) (sk: s_map) (tgm:t_map) (n: var)(* {struct lv} *): (exp_ctx * list var * var * t_map) :=
+           let fix convert_v_list (lv :list val_c) (sv : s_map) (sk: s_map) (tgm:conv_env) (n: var)(* {struct lv} *): (exp_ctx * list var * var * conv_env) :=
                match lv with
                  | nil => (Hole_c, nil, n, tgm)
                  | v::lv' =>
@@ -183,7 +235,7 @@ with convert_v (v:val_c) (sv: s_map) (sk: s_map) (tgm:t_map) (n:var) (* { struct
                end in
            let '(lv_ctx, nl, n', tgm) := convert_v_list lv sv sk tgm n in
            
-             (comp_ctx_f lv_ctx (Econstr_c n' (dcon_to_tag dcn) (List.rev nl) Hole_c), n', Pos.succ n', (M.set n' (dcon_to_tag dcn) tgm)) 
+             (comp_ctx_f lv_ctx (Econstr_c n' (dcon_to_tag dcn (fst tgm)) (List.rev nl) Hole_c), n', Pos.succ n', tgm) 
          | Fix_c lbt i =>
            (match lbt with
              | nil => (Hole_c, (1%positive), n, tgm) (* malformed input, should not happen *) 
@@ -206,15 +258,17 @@ arguments are:
 
 
  08/27/2016 - updated for directly-named functions in L5a instead of building a record
+ 09/08/2016 - now passing conv_env, containing a reverse cEnv to populate Econstr with the right cTag
  *)
-           let fix convert_fds (fds : list (list var * val_c))  (sv: s_map) (sk : s_map) (tgm:t_map) (fnames : list var) (n : var) (*{struct fds} *): (fundefs * var * t_map)  :=
+           let fix convert_fds (fds : list (list var * val_c))  (sv: s_map) (sk : s_map) (tgm:conv_env) (fnames : list var) (n : var) (*{struct fds} *): (fundefs * var * conv_env)  :=
                match (fds, fnames) with
                  | ((_,v)::fds', currn::fnames') =>
                    (match v with
                       | Lam_c x k e =>            
                         let '(ce, n', tgm) := convert e (M.set x n sv) (M.set k (Pos.succ n) sk) tgm (Pos.add n 2%positive) in
                         let '(cfds, n'', tgm) := convert_fds fds' sv sk tgm fnames' n' in
-                        (Fcons currn fun_tag (n::(Pos.succ n)::nil) ce cfds, n'', tgm)
+                        let (tgm1, tgm2) := tgm in 
+                        (Fcons currn fun_tag (n::(Pos.succ n)::nil) ce cfds, n'', (tgm1, M.set currn fun_tag tgm2))
                       | _ => (Fnil, n, tgm) (* this should not happen *)
                     end) 
                  | (_, _) => (Fnil, n, tgm)
@@ -226,8 +280,44 @@ arguments are:
              end)
        end.
 
-Definition convert_top (e:cps) : exp :=
-  let '(er, n, tgm) := convert e s_empty s_empty t_empty (3%positive) in er.
+
+Definition ienv := list (string * nat * itypPack).  
+
+Fixpoint convert_cnstrs (cct:list positive) (itC:list Cnstr) (ind:inductive) (nCon:N) (niT:iTag) ce (dcm:conId_map) :=
+ match (cct, itC) with  
+   | (cn::cct', cst::icT') =>
+     let (_, ccn) := cst in
+         convert_cnstrs cct' icT' ind (nCon+1)%N niT (M.set cn (niT, N.of_nat ccn, nCon) ce) (((ind,nCon), cn)::dcm)
+   | (_, _) => (ce, dcm)
+ end.
+               
+Fixpoint convert_typack typ (idBundle:string) (n:nat) (ice:(iEnv * cEnv* iTag * cTag * conId_map)) : (iEnv * cEnv * cTag * iTag * conId_map) :=
+  let '(ie, ce, niT, ncT, dcm) := ice in 
+  match typ with
+    | nil => ice
+    | (mkItyp itN itC ) ::typ' => 
+      let (cct, ncT) := fromN ncT (length itC) in
+      let (ce, dcm) := convert_cnstrs cct itC (mkInd idBundle n) 0 niT ce dcm in
+      let ityi := combine cct (map (fun (c:Cnstr) => let (_, n) := c in N.of_nat n) itC) in
+       convert_typack typ' idBundle (n+1) (M.set niT ityi ie, ce,  ncT, (Pos.succ niT), dcm)
+  end.
+      
+Fixpoint convert_env' (g:ienv) (ice:iEnv * cEnv * cTag * iTag * conId_map) : (iEnv * cEnv * conId_map) :=
+  let '(ie, ce, niT, ncT, dcm) := ice in 
+  match g with      
+    | nil => (ie, ce, dcm)
+    | (id, n, ty)::g' =>
+      (* id is name of mutual pack, n is number of type in mutual pack, ty is mutual pack *)
+      (* constructors are indexed with : name (string) of the mutual pack with which projection of the ty, and indice of the constructor *)      
+      convert_env' g' (convert_typack ty id 0 (ie, ce, ncT, niT, dcm)) 
+
+  end.
+
+Definition convert_env (g:ienv): (iEnv*cEnv * conId_map) := convert_env' g (M.empty iTyInfo, M.empty cTyInfo, 1%positive, 1%positive, nil).
+
+Definition convert_top (ee:ienv*cps) : (cEnv*exp) :=
+  let '(_, cG, dcm) := convert_env (fst ee) in 
+  let '(er, n, tgm) := convert (snd ee) s_empty s_empty (dcm, t_empty) (3%positive) in (cG, er).
 
 
 
